lang/Any.v
@@ -1,4 +1,5 @@
 Require Import sflib.
+Require Import Program.
 Require Import ClassicalDescription EquivDec.
 
 Set Implicit Arguments.
@@ -10,14 +11,47 @@ Hint Unfold Any.
 Definition excluded_middle_informative_extract_true := excluded_middle_informative.
 Extract Constant excluded_middle_informative_extract_true => "true".
 
-Definition try_type (a: Any) (T: Type): option T.
+Definition downcast (a: Any) (T: Type): option T.
   destruct a.
   destruct (excluded_middle_informative_extract_true (x = T)).
   - subst. apply Some. assumption.
   - apply None.
 Defined.
 
-Require Import Program.
+Definition upcast {T} (a: T): Any := existT id _ a.
+
+Lemma downcast_spec
+      a T t
+      (CAST: downcast a T = Some t)
+  :
+    <<TY: projT1 a = T>> /\ <<VAL: projT2 a ~= t>>
+.
+Proof.
+  unfold downcast in *. des_ifs. ss.
+  simpl_depind. eauto.
+Qed.
+
+Lemma downcast_intro
+      a T t
+      (TY: projT1 a = T)
+      (VAL: projT2 a ~= t)
+  :
+    <<CAST: downcast a T = Some t>>
+.
+Proof.
+  unfold downcast in *. des_ifs. ss.
+  dependent destruction e. ss.
+Qed.
+
+Lemma upcast_downcast
+      T (a: T)
+  :
+    downcast (upcast a) T = Some a
+.
+Proof.
+  eapply downcast_intro; ss.
+Qed.
+
 Definition Any_dec (a0 a1: Any): {a0=a1} + {a0<>a1}.
   destruct a0, a1.
   simpl_depind.
