hfc/Mpool.v
@@ -26,7 +26,7 @@ Import Monads.
 Import MonadNotation.
 Local Open Scope monad_scope.
 Local Open Scope string_scope.
-
+Require Import sflib.
 
 
 (* From HafniumCore *)
@@ -38,7 +38,7 @@ Set Implicit Arguments.
 
 
 
-Module MPOOL.
+Module MPOOLSEQ.
 
   (*
 Mpool := Vptr [Vptr//chunk_list ; Vptr//fallback]
@@ -46,43 +46,114 @@ Mpool := Vptr [Vptr//chunk_list ; Vptr//fallback]
 
   Definition entry_size: nat := 4096.
 
-  Definition p: string := "p".
-
-  Definition init (arg: val): stmt :=
-    p #:= arg#;
-
-      (Store p 0 Vnull)#;
-      (Store p 1 Vnull)#;
-
-      Skip
+  (* void init(struct mpool *p, size_t entry_size) *)
+  (* { *)
+  (*   p->entry_size = entry_size; *)
+  (*   p->chunk_list = NULL; *)
+  (*   p->entry_list = NULL; *)
+  (*   p->fallback = NULL; *)
+  (*   sl_init(&p->lock); *)
+  (* } *)
+  Definition init p: stmt :=
+    (Store p 0 Vnull) #;
+    (Store p 1 Vnull)
   .
 
-  (* Definition fini (arg: val): stmt := *)
-  (*   p #:= arg#; *)
+  (* void *mpool_alloc_contiguous(struct mpool *p, size_t count, size_t align) *)
+  (* { *)
+  (*   do { *)
+  (*     void *ret = mpool_alloc_contiguous_no_fallback(p, count, align); *)
+  
+  (*     if (ret != NULL) { *)
+  (*       return ret; *)
+  (*     } *)
+  
+  (*     p = p->fallback; *)
+  (*   } while (p != NULL); *)
+  
+  (*   return NULL; *)
+  (* } *)
+  Definition alloc_contiguous (p count ret: var): stmt :=
+    #while Vtrue
+     do (
+       ret #:= (Call "alloc_contiguous_no_fallback" [(p: expr) ; (count: expr)]) #;
+       #if (ret)
+       then (Return ret)
+       else Skip
+       fi #;
+       p #:= (Load p 1) #;
+       #if (p)
+       then Skip
+       else Break
+       fi
+     ) #;
+    Return Vnull
+  .
 
-  (*     #if (Load p 1) *)
-  (*           then *)
-  (*             else *)
-  (*               fi *)
-  (* . *)
+  (* void *mpool_alloc_contiguous_no_fallback(struct mpool *p, size_t count, *)
+  (*       				 size_t align) *)
+  (* { *)
+  (*   struct mpool_chunk **prev; *)
+  (*   void *ret = NULL; *)
+  
+  (*   align *= p->entry_size; *)
+  
+  (*   mpool_lock(p); *)
+  
+  (*   prev = &p->chunk_list; *)
+  (*   while ( *prev != NULL) { *)
+  (*     uintptr_t start; *)
+  (*     struct mpool_chunk *new_chunk; *)
+  (*     struct mpool_chunk *chunk = *prev; *)
+  
+  (*     start = (((uintptr_t)chunk + align - 1) / align) * align; *)
+  
+  (*     new_chunk = *)
+  (*       (struct mpool_chunk * )(start + (count * p->entry_size)); *)
+  (*     if (new_chunk <= chunk->limit) { *)
+  (*       if (new_chunk == chunk->limit) { *)
+  (*         *prev = chunk->next_chunk; *)
+  (*       } else { *)
+  (*         *new_chunk = *chunk; *)
+  (*         *prev = new_chunk; *)
+  (*       } *)
+  
+  (*       if (start - (uintptr_t)chunk >= p->entry_size) { *)
+  (*         chunk->next_chunk = *prev; *)
+  (*         *prev = chunk; *)
+  (*         chunk->limit = (struct mpool_chunk * )start; *)
+  (*       } *)
+  
+  (*       ret = (void * )start; *)
+  (*       break; *)
+  (*     } *)
+  
+  (*     prev = &chunk->next_chunk; *)
+  (*   } *)
+  
+  (*   mpool_unlock(p); *)
+  
+  (*   return ret; *)
+  (* } *)
+  Definition alloc_contiguous_no_fallback
+             (p count prev ret start new_chunk chunk: var): stmt :=
+    prev #:= (Load p 0) #;
+    #while prev
+     do (
+       ret #:= (Call "alloc_contiguous_no_fallback" [(p: expr) ; (count: expr)]) #;
+       #if (ret)
+       then (Return ret)
+       else Skip
+       fi #;
+       p #:= (Load p 1) #;
+       #if (p)
+       then Skip
+       else Break
+       fi
+     ) #;
+    Return Vnull
+  .
 
-  (* sum #:= Vnat 0#; *)
-  (* x #:= Vptr (repeat (Vnat 0) 3)#; *)
-  (* #put x#; *)
-  (* (Store x 0 10)#; *)
-  (* #put x#; *)
-  (* (Store x 1 20)#; *)
-  (* #put x#; *)
-  (* (Store x 2 30)#; *)
-  (* #put x#; *)
-  (* #put sum#; *)
-  (* sum #:= sum + (Load x 0)#; *)
-  (* #put sum#; *)
-  (* sum #:= sum + (Load x 1)#; *)
-  (* #put sum#; *)
-  (* sum #:= sum + (Load x 2)#; *)
-  (* #put sum#; *)
-  (* Skip *)
 
-End MPOOL.
+End MPOOLSEQ.
 
